Work in progress ...

Isabelle/Grammar.thy
@@ -61,8 +61,7 @@ definition norm_list_of_rules ::
 definition norm_of_production_rules ::
   "('t :: linorder, 'v :: linorder) grammar \<Rightarrow> ('t, 'v) norm_list" where
   "norm_of_production_rules gr \<equiv> (fold (\<lambda>(v, rules). \<lambda>norms.
-     let min_norm = Min (set (norm_list_of_rules norms rules)) in
-     norms@[(v, min_norm)]) gr [])"
+     norms@[(v, Min (set (norm_list_of_rules norms rules)))]) gr [])"
 
 fun eat_word :: "('t, 'v) grammar \<Rightarrow> 't list \<Rightarrow> 'v list \<Rightarrow> ('t list \<times> 'v list)" where
   "eat_word gr (th#tt) (vh#vt) = (
@@ -191,6 +190,10 @@ by (auto simp add: norm_of_production_rules_def
 lemma "norm_list_of_rules norms rules = l \<Longrightarrow> snd ` set l \<subseteq> set rules"
 by (unfold norm_list_of_rules_def) auto
 
+lemma nlor_nonempty:
+  "\<exists>(t, vs) \<in> set rules. \<forall>v \<in> set vs. v \<in> fst ` set norms \<Longrightarrow> norm_list_of_rules norms rules \<noteq> []"
+by (auto simp add: norm_list_of_rules_def filter_empty_conv)
+
 lemma nopr_fst_is_gr_fst:
   "(v, n, t, vs) \<in> set (norm_of_production_rules gr) \<Longrightarrow> v \<in> fst ` set gr"
   apply (rule subst [of "set (map fst gr)"])
@@ -226,6 +229,53 @@ proof -
   then show ?thesis using L by simp
 qed
 
+thm helper3' [of "(\<lambda>(v, rules) norms. norms @ [(v, Min (set (norm_list_of_rules norms rules)))])"
+                           "\<lambda>(v, rules) norms. (v, Min (set (norm_list_of_rules norms rules)))"
+                           "\<lambda>(v, n, t, vs). t \<in> fst ` set (of_key gr v)" "(v, n, t, vs)" gr]
+
+thm fold_invariant[of gr "\<lambda>(v, rules). of_key gr v = rules"
+  "\<lambda>s. \<forall>(v, n, t, vs) \<in> set s. t \<in> fst ` set (of_key gr v)" "[]" "(\<lambda>(v, rules) norms. norms @ [(v, Min (set (norm_list_of_rules norms rules)))])"]
+
+lemma
+  assumes G: "gram_valid gr"
+      and N: "(v, n, t, vs) \<in> set (norm_of_production_rules gr)"
+    shows "(t, vs) \<in> set (of_key gr v)"
+proof -
+  have XX: "\<forall>(k, v)\<in>set gr. is_alist v" using G by (auto simp add: gram_valid_def is_typical_alist_def)
+  have XY: "v \<in> fst ` set gr" using G N by (simp add: nopr_fst_is_gr_fst)
+  have AL: "is_alist (of_key gr v)" using XX XY by (rule of_key_forall)
+
+  have T1: "\<And>x. gram_valid gr \<Longrightarrow> x \<in> set gr \<Longrightarrow> case x of (v, rules) \<Rightarrow> of_key gr v = rules"
+    by (auto simp add: of_key_from_existence gram_valid_def is_typical_alist_def)
+  have T2: "\<And>P. \<forall>x\<in>set []. P x" by auto
+
+  have ABC: "\<And>a norms. \<forall>(v, n, t, vs)\<in>set norms. t \<in> fst ` set (of_key gr v) \<Longrightarrow>
+             \<exists>(n, t, vs) \<in> (set (norm_list_of_rules norms (of_key gr a))). True" sorry
+
+  have XYZ: "\<And>a s ab ac ba. \<forall>(v, n, t, vs)\<in>set s. t \<in> fst ` set (of_key gr v) \<Longrightarrow>
+             (ab, ac, ba) = Min (set (norm_list_of_rules s (of_key gr a))) \<Longrightarrow>
+             ac \<in> fst ` set (of_key gr a)" using G ABC by (auto simp add: Min.closed nlor_nonempty norm_list_of_rules_def) (* TODO! *)
+
+  have T3: "\<And>x s. gram_valid gr \<Longrightarrow>
+          case x of (v, rules) \<Rightarrow> of_key gr v = rules \<Longrightarrow>
+          \<forall>(v, n, t, vs)\<in>set s. t \<in> fst ` set (of_key gr v) \<Longrightarrow>
+          \<forall>(v, n, t, vs)\<in>set ((\<lambda>(v, rules) norms. norms @ [(v, Min (set (norm_list_of_rules norms rules)))]) x s).
+             t \<in> fst ` set (of_key gr v)" using G XYZ by auto
+
+  have SGX: "gram_valid gr \<Longrightarrow>
+    \<forall>(v, n, t, vs)\<in>set (norm_of_production_rules gr).
+      t \<in> fst ` set (of_key gr v)" unfolding norm_of_production_rules_def using T1 T2 T3
+    by (rule fold_invariant[of _ "\<lambda>(v, rules). of_key gr v = rules"
+      "\<lambda>s. \<forall>(v, n, t, vs) \<in> set s. t \<in> fst ` set (of_key gr v)" _])
+
+  have SG: "\<forall>(v, n, t, vs) \<in> set (norm_of_production_rules gr). t \<in> fst ` set (of_key gr v)"
+    using G SGX by (auto simp add: norm_of_production_rules_def)
+
+  have EX1: "t \<in> fst ` set (of_key gr v)" using N SG by auto
+  have EX2: "of_key (of_key gr v) t = vs" sorry
+  show ?thesis using AL EX1 EX2 by (rule existence_from_of_key)
+qed
+
 lemma "gram_valid gr \<Longrightarrow> (v, n, t, vs) \<in> set (norm_of_production_rules gr) \<Longrightarrow>
   (t, vs) \<in> set (of_key gr v)"
   apply (rule existence_from_of_key)
@@ -233,6 +283,15 @@ lemma "gram_valid gr \<Longrightarrow> (v, n, t, vs) \<in> set (norm_of_producti
   apply (simp add: gram_valid_def is_typical_alist_def)
   apply (auto simp add: nopr_fst_is_gr_fst)
   apply (auto simp add: norm_of_production_rules_def)
+  apply (subgoal_tac "\<forall>(v, n, t, vs) \<in> set (fold (\<lambda>(v, rules) norms. norms @ [(v, Min (set (norm_list_of_rules norms rules)))]) gr []). t \<in> fst ` set (of_key gr v)")
+  apply auto[1]
+  apply (thin_tac "(v, n, t, vs) \<in> set (fold (\<lambda>(v, rules) norms. norms @ [(v, Min (set (norm_list_of_rules norms rules)))]) gr [])")
+  apply (rule fold_invariant[of _ "\<lambda>(v, rules). of_key gr v = rules"
+  "\<lambda>s. \<forall>(v, n, t, vs) \<in> set s. t \<in> fst ` set (of_key gr v)" _])
+  apply (auto simp add: of_key_from_existence gram_valid_def is_typical_alist_def)
+  apply auto
+  apply (auto elim: Min.closed)
+
   apply (subgoal_tac "case (v, n, t, vs) of (v, n, t, vs) \<Rightarrow> t \<in> fst ` set (of_key gr v)")
   apply simp
   apply (rule helper3' [of "(\<lambda>(v, rules) norms. norms @ [(v, Min (set (norm_list_of_rules norms rules)))])"
